books/kestrel/remora/abstract-syntax-constructors.lisp
@@ -135,102 +135,6 @@
           from dimensions and shapes to concatenate."
   `(shape-append (list ,@(shape-terms-from-vars/dims/others dims/shapes))))
 
-;;;;;;;;;;;;;;;;;;;;;;;;;;;;;;;;;;;;;;;;;;;;;;;;;;;;;;;;;;;;;;;;;;;;;;;;;;;;;;;;
-
-(define atom-type-term-from-var/base/other (type)
-  :short "Construct an atom type term from
-          a string denoting an atom type variable,
-          or a keyword denoting a base type,
-          or some other term that is left unchanged."
-  :long
-  (xdoc::topstring
-   (xdoc::p
-    "The string denoting a variable must start with @('&')."))
-  (cond ((stringp type)
-         (b* (((mv & name) (var-string-split type '(#\&))))
-           `(atom-type-var ,name)))
-        ((eq type :bool) '(atom-type-base (base-type-bool)))
-        ((eq type :int) '(atom-type-base (base-type-int)))
-        ((eq type :float) '(atom-type-base (base-type-float)))
-        (t type)))
-
-;;;;;;;;;;;;;;;;;;;;
-
-(define atom-type-terms-from-vars/bases/others ((types true-listp))
-  :short "Lift @(tsee atom-type-term-from-var/base/other) to lists."
-  (cond ((endp types) nil)
-        (t (cons (atom-type-term-from-var/base/other (car types))
-                 (atom-type-terms-from-vars/bases/others (cdr types))))))
-
-;;;;;;;;;;;;;;;;;;;;;;;;;;;;;;;;;;;;;;;;
-
-(defmacro+ t[] (type dim/shape)
-  :short "Construct an array type term from the element type and the shape."
-  :long
-  (xdoc::topstring
-   (xdoc::p
-    "Strings, natural numbers, and base type keywords
-     are auto-coerced to ispaces and types."))
-  `(array-type-array ,(atom-type-term-from-var/base/other type)
-                     ,(shape-term-from-var/dim/other dim/shape)))
-
-;;;;;;;;;;;;;;;;;;;;;;;;;;;;;;;;;;;;;;;;
-
-(define array-type-term-from-var/atom/other (type)
-  :short "Construct an array type term from
-          a string denoting an atom or array type variable,
-          or a keyword denoting a base type,
-          or a function type term,
-          or a universal type term,
-          or a product type term,
-          or a sum type term,
-          or some other term that is left unchanged."
-  :long
-  (xdoc::topstring
-   (xdoc::p
-    "The string denoting a variable must start with @('&') or @('*').")
-   (xdoc::p
-    "An atom type is turned into an array type by adding an empty shape."))
-  (cond ((stringp type)
-         (b* (((mv prefix name) (var-string-split type '(#\& #\*))))
-           (case prefix
-             (#\& `(array-type-array (atom-type-var ,name) (shape)))
-             (#\* `(array-type-var ,name)))))
-        ((eq type :bool) '(array-type-array (atom-type-base (base-type-bool))
-                                            (shape)))
-        ((eq type :int) '(array-type-array (atom-type-base (base-type-int))
-                                           (shape)))
-        ((eq type :float) '(array-type-array (atom-type-base (base-type-float))
-                                             (shape)))
-        ((and (consp type) (eq (car type) 't->))
-         `(array-type-array ,type (shape)))
-        ((and (consp type) (eq (car type) 'tforall))
-         `(array-type-array ,type (shape)))
-        ((and (consp type) (eq (car type) 'tpi))
-         `(array-type-array ,type (shape)))
-        ((and (consp type) (eq (car type) 'tsigma))
-         `(array-type-array ,type (shape)))
-        (t type)))
-
-;;;;;;;;;;;;;;;;;;;;
-
-(define array-type-terms-from-vars/atoms/others ((types true-listp))
-  :short "Lift @(tsee array-type-term-from-var/atom/other) to lists."
-  (cond ((endp types) nil)
-        (t (cons (array-type-term-from-var/atom/other (car types))
-                 (array-type-terms-from-vars/atoms/others (cdr types))))))
-
-;;;;;;;;;;;;;;;;;;;;;;;;;;;;;;;;;;;;;;;;
-
-(defmacro+ t-> (intypes outtype)
-  :short "Construct a function type term from the input and output types."
-  :long
-  (xdoc::topstring
-   (xdoc::p
-    "Strings and base type keywords are auto-coerced to types."))
-  `(atom-type-fun (list ,@(array-type-terms-from-vars/atoms/others intypes))
-                  ,(array-type-term-from-var/atom/other outtype)))
-
 ;;;;;;;;;;;;;;;;;;;;;;;;;;;;;;;;;;;;;;;;
 
 (define ispace-var-term-from-string ((str stringp))
@@ -252,7 +156,7 @@
         (t (cons (ispace-var-term-from-string (car strs))
                  (ispace-var-terms-from-strings (cdr strs))))))
 
-;;;;;;;;;;;;;;;;;;;;;;;;;;;;;;;;;;;;;;;;
+;;;;;;;;;;;;;;;;;;;;;;;;;;;;;;;;;;;;;;;;;;;;;;;;;;;;;;;;;;;;;;;;;;;;;;;;;;;;;;;;
 
 (define type-var-term-from-string ((str stringp))
   :short "Build a type variable term from a string."
@@ -275,12 +179,60 @@
 
 ;;;;;;;;;;;;;;;;;;;;;;;;;;;;;;;;;;;;;;;;
 
+(define type-term-from-var/base/other (type)
+  :short "Construct a type term from
+          a string denoting an atom type variable,
+          or a keyword denoting a base type,
+          or some other term that is left unchanged."
+  :long
+  (xdoc::topstring
+   (xdoc::p
+    "The string denoting a variable must start with @('&') or @('*')."))
+  (cond ((stringp type) `(type-var ,(type-var-term-from-string type)))
+        ((eq type :bool) '(type-array (type-base (base-type-bool)) (shape)))
+        ((eq type :int) '(type-array (type-base (base-type-int)) (shape)))
+        ((eq type :float) '(type-array (type-base (base-type-float)) (shape)))
+        (t type)))
+
+;;;;;;;;;;;;;;;;;;;;
+
+(define type-terms-from-vars/bases/others ((types true-listp))
+  :short "Lift @(tsee type-term-from-var/base/other) to lists."
+  (cond ((endp types) nil)
+        (t (cons (type-term-from-var/base/other (car types))
+                 (type-terms-from-vars/bases/others (cdr types))))))
+
+;;;;;;;;;;;;;;;;;;;;;;;;;;;;;;;;;;;;;;;;
+
+(defmacro+ t[] (type dim/shape)
+  :short "Construct a type term from the element type and the shape."
+  :long
+  (xdoc::topstring
+   (xdoc::p
+    "Strings, natural numbers, and base type keywords
+     are auto-coerced to ispaces and types."))
+  `(type-array ,(type-term-from-var/base/other type)
+               ,(shape-term-from-var/dim/other dim/shape)))
+
+;;;;;;;;;;;;;;;;;;;;;;;;;;;;;;;;;;;;;;;;
+
+(defmacro+ t-> (intypes outtype)
+  :short "Construct a function type term from the input and output types."
+  :long
+  (xdoc::topstring
+   (xdoc::p
+    "Strings and base type keywords are auto-coerced to types."))
+  `(type-fun (list ,@(type-terms-from-vars/bases/others intypes))
+             ,(type-term-from-var/base/other outtype)))
+
+;;;;;;;;;;;;;;;;;;;;;;;;;;;;;;;;;;;;;;;;
+
 (defmacro+ tforall (params type)
   :short "Construct a universal type from
           a parenthesized list of variable strings (parameters)
           and a type term (body)."
-  `(atom-type-forall (list ,@(type-var-terms-from-strings params))
-                     ,(array-type-term-from-var/atom/other type)))
+  `(type-forall (list ,@(type-var-terms-from-strings params))
+                ,(type-term-from-var/base/other type)))
 
 ;;;;;;;;;;;;;;;;;;;;;;;;;;;;;;;;;;;;;;;;
 
@@ -288,8 +240,8 @@
   :short "Construct a product type term from
           a parenthesized list of variable strings (parameters)
           and a type type (body)."
-  `(atom-type-pi (list ,@(ispace-var-terms-from-strings params))
-                 ,(array-type-term-from-var/atom/other type)))
+  `(type-pi (list ,@(ispace-var-terms-from-strings params))
+            ,(type-term-from-var/base/other type)))
 
 ;;;;;;;;;;;;;;;;;;;;;;;;;;;;;;;;;;;;;;;;
 
@@ -297,5 +249,5 @@
   :short "Construct a sum type term from
           a parenthesized list of variable strings (parameters)
           and a type type (body)."
-  `(atom-type-sigma (list ,@(ispace-var-terms-from-strings params))
-                    ,(array-type-term-from-var/atom/other type)))
+  `(type-sigma (list ,@(ispace-var-terms-from-strings params))
+               ,(type-term-from-var/base/other type)))
