books/kestrel/remora/static-environments.lisp
@@ -33,11 +33,7 @@
      the sort environment @($\\Theta$),
      the kind environment @($\\Delta$), and
      the type environment @($\\Gamma$)
-     in [arxiv], [thesis], and [esop].")
-   (xdoc::p
-    "This is currently not used in the type checker.
-     It is intended for use in the upcoming declarative typing rules.
-     We may also use it in the type checker."))
+     in [arxiv], [thesis], and [esop]."))
   :order-subtopics t
   :default-parent t)
 
@@ -61,17 +57,17 @@
       but since our type variables include their own kind,
       a set suffices, as opposed to a map from variables to kinds.")
     (xdoc::li
-     "A map from the expression variables in scope to their array types.
+     "A map from the expression variables in scope to their types.
       This corresponds to @($\\Gamma$).")))
   ((ispace-vars ispace-var-set)
    (type-vars type-var-set)
-   (expr-vars string-arraytype-map))
+   (expr-vars string-type-map))
   :pred senvp)
 
 ;;;;;;;;;;;;;;;;;;;;;;;;;;;;;;;;;;;;;;;;;;;;;;;;;;;;;;;;;;;;;;;;;;;;;;;;;;;;;;;;
 
 (define prim-op-types ()
-  :returns (term-vars string-arraytype-mapp)
+  :returns (term-vars string-type-mapp)
   :short "Association of primitive operations to their types."
   :long
   (xdoc::topstring
@@ -134,7 +130,7 @@
 
 ;;;;;;;;;;;;;;;;;;;;;;;;;;;;;;;;;;;;;;;;;;;;;;;;;;;;;;;;;;;;;;;;;;;;;;;;;;;;;;;;
 
-(define senv-add-var+type ((var stringp) (type array-typep) (senv senvp))
+(define senv-add-var+type ((var stringp) (type typep) (senv senvp))
   :returns (new-senv senvp)
   :short "Add a variable with a type to the static environment."
   :long
@@ -144,7 +140,7 @@
      which is intended hiding behavior."))
   (b* ((expr-vars (senv->expr-vars senv))
        (new-expr-vars (omap::update (str::str-fix var)
-                                    (array-type-fix type)
+                                    (type-fix type)
                                     expr-vars)))
     (change-senv senv :expr-vars new-expr-vars)))
 
